src/HOL/Bali/Type.thy
@@ -36,8 +36,9 @@ abbreviation "Class C == RefT (ClassT C)"
 abbreviation Array :: "ty \<Rightarrow> ty"  ("_.[]" [90] 90)
   where "T.[] == RefT (ArrayT T)"
 
-definition the_Class :: "ty \<Rightarrow> qtname" where
- "the_Class T \<equiv> SOME C. T = Class C" (** primrec not possible here **)
+definition
+  the_Class :: "ty \<Rightarrow> qtname"
+  where "the_Class T = (SOME C. T = Class C)" (** primrec not possible here **)
  
 lemma the_Class_eq [simp]: "the_Class (Class C)= C"
 by (auto simp add: the_Class_def)
